theories/Block/vst/verif/certicoq_block__init.v
@@ -1,0 +1,28 @@
+From VST Require Import floyd.proofauto.
+
+From CertiCoq Require Import Block.vst.ast.ast.
+From CertiCoq Require Import Block.vst.clightgen.block.
+From CertiCoq Require Import Block.vst.cmodel.certicoq_block_header.
+From CertiCoq Require Import Block.vst.cmodel.certicoq_block.
+From CertiCoq Require Import Block.vst.spec.spec.
+
+Lemma body: semax_body Vprog ASI f_certicoq_block__init certicoq_block__init_spec.
+Proof.
+  start_function.
+  unfold block_header_size, block_header_at, undef_block_at.
+  Intros.
+  forward.
+  forward.
+  forward.
+  {
+    entailer!.
+    pose proof (block_header_field_count__range h) as HH1.
+    lia.
+  }
+  forward.
+  {
+    entailer!.
+    unfold block_at, block_header_at, block_fields_at.
+    admit.
+  }
+Admitted.
